start.sh
@@ -1,2 +1,2 @@
 #! /bin/bash
-~/Isabelle2024/bin/isabelle jedit -d BridgeDefinition -l BridgeDefinition
+~/Isabelle2024/bin/isabelle jedit -d BridgeProperties -d BridgeDefinition -l BridgeProperties
